\only<1>{
\Def{Equational Theory: Computation Laws}
    {
     \vspace*{-0.3cm}
     \[ (\lambda \alpha. M) \; N = M[id, N : \alpha] \]
     \vspace*{-0.3cm}
    }
\Ex{Beta Reduction}
    {Application reduces by substituting the argument}
}

\only<2>{
\Def{Equational Theory: Computation Laws}
    {
     \vspace*{-0.3cm}
     \[ (\lambda \alpha. M) \; N = M[id, N : \alpha] \]
     \vspace*{-0.3cm}
     \[ M = \lambda \alpha. (M[\uparrow] \; 1) \]
     \vspace*{-0.3cm}
    }
\Ex{Eta Expansion}
    {Any term can be eta-expanded by shifting and applying to variable 1}
}

\only<3>{
\Def{Equational Theory: Computation Laws}
    {
     \vspace*{-0.3cm}
     \[ (\lambda \alpha. M) \; N = M[id, N : \alpha] \]
     \vspace*{-0.3cm}
     \[ M = \lambda \alpha. (M[\uparrow] \; 1) \]
     \vspace*{-0.3cm}
     \[ 1[id, M : \alpha] = M \]
     \vspace*{-0.3cm}
    }
\Ex{Variable Beta}
    {Substituting for variable 1 with extension gives the substituted term}
}
