\only<1>{
\Def{Equational Theory: Distribution Laws}
    {
     \vspace*{-0.3cm}
     \[ (M \; N)[\gamma] = M[\gamma] \; N[\gamma] \]
     \vspace*{-0.3cm}
    }
\Ex{Application Distribution}
    {Substitution distributes over application.}
}

\only<2>{
\Def{Equational Theory: Distribution Laws}
    {
     \vspace*{-0.3cm}
     \[ (M \; N)[\gamma] = M[\gamma] \; N[\gamma] \]
     \vspace*{-0.3cm}
     \[ (\lambda \alpha. M)[\gamma] = \lambda \alpha. M[(\uparrow \circ \gamma), 1 : \alpha] \]
     \vspace*{-0.3cm}
    }
\Ex{Abstraction Distribution}
    {Substitution distributes under binders by extending a weakening with variable.}
}

