\only<1>{
\Def{Equational Theory: Composition Laws}
    {
     \vspace*{-0.3cm}
     \[ 1[\gamma] = \gamma_1 \]
     \vspace*{-0.3cm}
    }
\Ex{Variable Substitution}
    {Substituting into variable 1 extracts the first component of the substitution}
}

\only<2>{
\Def{Equational Theory: Composition Laws}
    {
     \vspace*{-0.3cm}
     \[ 1[\gamma] = \gamma_1 \]
     \vspace*{-0.3cm}
     \[ (M \; N)[\gamma] = M[\gamma] \; N[\gamma] \]
     \vspace*{-0.3cm}
    }
\Ex{Application Distribution}
    {Substitution distributes over application}
}

\only<3>{
\Def{Equational Theory: Composition Laws}
    {
     \vspace*{-0.3cm}
     \[ 1[\gamma] = \gamma_1 \]
     \vspace*{-0.3cm}
     \[ (M \; N)[\gamma] = M[\gamma] \; N[\gamma] \]
     \vspace*{-0.3cm}
     \[ (\lambda \alpha. M)[\gamma] = \lambda \alpha. M[\gamma^+] \]
     \vspace*{-0.3cm}
    }
\Ex{Abstraction Distribution}
    {Substitution under lambda requires lifting: $\gamma^+ = (\gamma \circ \uparrow, 1)$}
}

\only<4>{
\Def{Equational Theory: Composition Laws}
    {
     \vspace*{-0.3cm}
     \[ 1[\gamma] = \gamma_1 \]
     \vspace*{-0.3cm}
     \[ (M \; N)[\gamma] = M[\gamma] \; N[\gamma] \]
     \vspace*{-0.3cm}
     \[ (\lambda \alpha. M)[\gamma] = \lambda \alpha. M[\gamma^+] \]
     \vspace*{-0.3cm}
     \[ M[\gamma][\delta] = M[\gamma \circ \delta] \]
     \vspace*{-0.3cm}
    }
\Ex{Substitution Composition}
    {Sequential substitution equals composition}
}
